\section*{Mathematical Analysis IIIA:}


\section*{1. Linear Ordinary Differential Equations}

\subsection*{First Order Linear Equations}
$y'+p(x)y=g(x)$:
\begin{align*}
 y(x) &= e^{-M(x)}\left(C+\int g(x) e^{M(x)}\, dx\right),
 & \text{where } M(x) = \int p(x) dx.
\end{align*}

\subsection*{Reduction of order}
$y'' + p(x)y' + q(x)y=0$:
\begin{align*}
 u_2(x)&= u_1(x) \int \frac{e^{-P(t)}}{u_1^2(t)}\, dt, 
&\text{where } P(x) =  \int p(x)\, dx.
\end{align*}

\subsection*{Shift rule}
\[
    P(D) (e^{\lambda x}f(x)) = e^{\lambda x}P(D+\lambda)f(x)
\]
 
\subsection*{Green function}
Solution to $y^{(n)} + p_{n-1}(x)y^{(n-1)}+\cdots+p_1(x)y'+p_0y=g(x)$,
$U_1(y)=U_2(y)=\cdots=U_n(y)=0$,
\[
  y(x) = \int_a^b G(x,\xi) g(\xi)\, d\xi.
  \]

\section*{2. Separation of Variables}

\subsection*{Newton's equation}
Equation: $x''=F(x)$ or  $(\{x'=y,y'=F(x)\})$.\\
Potential: $U(x) := -\int F(x)\, dx$.\\
Energy: $E(x,y) := U(x) + \frac {y^2}2$.\\
Period of small oscillations: $\lim_{\epsilon \to 0} L_\epsilon = 
\frac{2\pi}{\sqrt{U''(x_0)}}$.

\section*{3. Series Solutions of Linear Equations}

\subsection*{Recursive formula for the coefficients at an ordinary point}
\begin{align*}
    (k+2)(k+1)c_{k+2} + \sum_{j=0}^{k} (k-j+1)a_jc_{k-j+1} + \sum_{j=0}^{k}b_jc_{k-j} &= 0. 
\end{align*}

\subsection*{Recursive formula for the coefficients at a regular singular point}
\begin{align*}
P(k+\gamma)c_k + \sum_{j=0}^{k-1} ((j+\gamma)a_{k-j} + b_{k-j}) c_j &=0, &k\in \mathbb N,
\end{align*}
with the understanding that for $k=0$ the sum is empty, and the indicial 
polynomial $P$ is given by 
\begin{align*}
 P(X) &= X(X-1) + a_0X + b_0.
\end{align*}

\section*{4. Existence Theory}

\subsection*{Picard iteration}
\begin{align*}
  \phi_{m+1}(x) = y_0 + \int_{x_0}^x f(t,\phi_m(t))\, dt.
\end{align*}

\section*{5. The Exponential of a Matrix}

Solution to $y'=A(x)y+h(x)$, $y(x_0)=\eta$ is 
$y(x) = e^{(x-x_0)A}\eta + \int_{x_0}^x e^{(x-t)A}h(t)\, dt$.

\subsection*{Newton divided differences}
\[
    F[\lambda_l] = F(\lambda_l), \qquad
    F[\lambda_l,\ldots,\lambda_{l+k}] = 
    \frac{F[\lambda_l+1,\ldots,\lambda_{l+k}]-F[\lambda_l,\ldots,
    \lambda_{l+k-1}]}{\lambda_{l+k}-\lambda_l}.
\]
If $\lambda_l=\cdots = \lambda_{k+l}$, then 
$F[\lambda,\ldots,\lambda_{l+k}] = F^{(k)}(\lambda_l)/k!$.


\section*{7. Sturm-Liouville Theory}

\subsection*{Sturm-Liouville form}
\begin{align*}
 Ly = \frac{d}{dx} \left(p(x)\frac{dy}{dx}\right) + q(x)y = g(x).
\end{align*}

\subsection*{Inner product, norm and Bessel inequality}
\begin{align*}
 \langle u,v\rangle &= \int_a^b u(x)\overline {v(x)}\, dx, 
 \qquad \qquad  \|u\|_2 = \sqrt{\langle u,u\rangle },
 \qquad \qquad \sum_{n=1}^{\infty} |\langle f, \phi_n\rangle|^2 \leq 
 \|f\|_2^2.
\end{align*}

\subsection*{Solutions to non-homogeneous equations}
\begin{center}$Ly-\mu y = h(x)$, $U_1(y)=0$, $U_2(y)=0$. \end{center}
If $\mu$ not an eigenvalue: $y(x) = \sum_{n=1}^\infty (\lambda_n- \mu)^{-1}\langle h,\phi_n 
\rangle \phi_n(x)$.\\
If $\mu$ is an eigenvalue: $y(x) = \sum_{\lambda_n\neq \mu}^\infty (\lambda_n - \mu)^{-1}\langle h,\phi_n 
\rangle \phi_n(x)$.

\section*{Fourier Analysis}

 \subsection*{Fourier series $f$ on $[-L,L]$: Exponential form:}
 
 \begin{align*}
  f(x) &\sim \frac{c_0}2 + \sum_{n=-\infty}^\infty c_n e^{\frac{inx\pi}{L},}\\
  c_n &= \hat f(n) = \frac 1{2L} \int_{-L}^L f(x) e^{-\frac{in\pi x}L}\, dx, \qquad n\in \mathbb Z.
 \end{align*}


 \subsection*{Fourier series $f$ on $[-L,L]$: Trigonometric form}

   \[
  f(x) \sim \frac{a_0}2 + \sum_{n=1}^\infty a_n \cos\left(\frac {n\pi x}L \right) + 
  \sum_{n=1}^{\infty}b_n \sin\left(\frac{n\pi x}L \right).
 \]
  \begin{align*}
   a_n &= \frac 1L \int_{-L}^{L} f(x) \cos\left(\frac{n\pi x}L\right)\, dx, \quad n\geq 0.
  &b_n = \frac 1L \int_{-L}^L f(x) \sin\left(\frac{n\pi x}L \right)\, dx, \quad n\geq 1.
 \end{align*}

 \subsection*{Connections between coefficients:}
 \begin{minipage}{.45\linewidth}
    \begin{align*}
    c_0 &= a_0,\\
    c_n &= (a_n-ib_n)/2, &\text{for } n>0,\\
    c_n &= (a_{-n} + ib_{-n})/2, &\text{for } n<0.
    \end{align*}
  \end{minipage}%
  \begin{minipage}{.45\linewidth}
    \begin{align*}
    a_0 &= c_0,\\
    a_n &= c_n + c_{-n}, &\text{for } n>0,\\
    b_n &= i(c_n - c_{-n}), &\text{for } n>0.
    \end{align*}
  \end{minipage}%

 \subsection*{Solving Ordinary Differential Equations}
  If $P(D)u=f$, then $P(in)\hat u(n) = \hat f(n)$ and
\[ u(x) = \sum_{n=-\infty}^{\infty} \frac{\hat f(n)}{P(in)}e^{inx}.\]
 
